

# Calculus of ordinary generating functions (o.g.f.)

$$f(x) = \sum_n a_n x^n \Rightarrow f'(x) \triangleq \sum_{n \geq 1} n a_n x^{n-1} \quad (\text{The formal derivative})$$

$$\bullet (f(x)g(x))' = f'(x)g(x) + f(x)g'(x) \quad (\text{product rule})$$

$$\bullet (f(g(x)))' = f'(g(x))g'(x) \quad (\text{chain rule})$$

$$\bullet \text{ if } f' = 0, \text{ Then } f \text{ is a constant} \quad \leftarrow [\text{integration makes sense}]$$

$$\bullet f' = f \Rightarrow f = a \cdot e^x \quad \leftarrow \begin{array}{l} \text{We will use} \\ D \text{ for the differential} \\ \text{operator.} \end{array}$$

We're associating sequences to their o.g.f's:

$$\{a_n\}_{n \in \mathbb{N}} \xleftrightarrow{\text{o.g.f.}} f(x) = \sum_{n \geq 0} a_n x^n, \quad \{b_n\}_{n \in \mathbb{N}} \xleftrightarrow{\text{o.g.f.}} g$$

$$\bullet \{a_{n+h}\}_{n \in \mathbb{N}} \longleftrightarrow (f - \sum_{m=0}^{h-1} a_m x^m) / x^h \quad (\text{shifting})$$

$$\bullet \{a_n + b_n\}_{n \in \mathbb{N}} \longleftrightarrow f + g \quad (\text{sum})$$

$$\bullet \{n a_n\}_{n \in \mathbb{N}} \longleftrightarrow x \cdot D f \quad \text{operator}$$

$$\text{In general } \left[ \{p(n) a_n\}_{n \in \mathbb{N}} \longleftrightarrow p(x \cdot D) f \right]$$

**Example** Let  $f(x) = 1 + x + \dots + x^m = \frac{x^{m+1} - 1}{x - 1}$

$$\text{Then } g(x) = \sum_{j=0}^m j^n x^j = (xD)^n f(x)$$

$$\Rightarrow \sum_{j=0}^m j^n = (xD)^n \frac{x^{m+1} - 1}{x - 1} \Big|_{x=1}$$

$$\bullet \left\{ \sum_{k=0}^m a_k b_{m-k} \right\}_{m \in \mathbb{N}} \longleftrightarrow fg \quad (\text{product})$$

$$\bullet \left\{ \sum_{m_1 + \dots + m_k = m} a_{m_1} \dots a_{m_k} \right\}_{m \in \mathbb{N}} \longleftrightarrow f^k \quad (\text{power})$$

**Example**  $\frac{1}{(1-x)^n} = \sum_{m \geq 0} \left( \sum_{m+k=m} 1 \right) x^m = \sum_{m \geq 0} \binom{n+k-1}{m} x^m$

•  $\left[ \frac{1}{1-x} \right] \longleftrightarrow \left\{ \sum_{k=0}^m a_k \right\}_{m \geq 0}$  (partial sums)

**Example**  $\sum_{k=0}^m F_k = F_{m+2} - 1$

$\frac{1}{1-x} F(x) = \frac{x}{(1-x)(1-x-x^2)}$  ✓

$\frac{F(x)-x}{x^2} = \frac{1}{1-x}$

$= \frac{1}{x^2} \left( \frac{x}{1-x-x^2} - x \right) = \frac{1}{1-x}$

$= \frac{x}{(1-x)(1-x-x^2)}$  ✓

**Example**  $\sum_{m,k} \binom{m}{k} x^k y^m = \frac{1}{1-(x+1)y} \Rightarrow$

$\Rightarrow x \sum_{m,k} \binom{m}{k} x^k x^m = \frac{x}{1-x-x^2} = \sum_{m \geq 0} F_m x^m \Rightarrow$

$\Rightarrow \left[ F_r \right] = \sum_{m+k=r-1} \binom{m}{k}$

Let  $A(m, k) = \# \{ \text{set partitions of } [m] \text{ into } k \text{ non-empty parts} \}$

Example  $m=3$

$$\bullet A(3, 1) = 1 \quad \{ \{ \{1, 2, 3\} \} \}$$

$$\bullet A(3, 2) = \{ \{ \{1, 2\}, \{3\} \}, \{ \{1, 3\}, \{2\} \}, \{ \{2, 3\}, \{1\} \} \}$$

$$\bullet A(3, 3) = \{ \{ \{1\}, \{2\}, \{3\} \} \}$$

We use  $\left\{ \begin{smallmatrix} m \\ k \end{smallmatrix} \right\} \triangleq |A(m, k)|$  (Stirling numbers of the second kind)

$$\bullet \left\{ \begin{smallmatrix} m \\ k \end{smallmatrix} \right\} = 0 \quad \text{for } k > m, \quad \bullet \left\{ \begin{smallmatrix} m \\ 0 \end{smallmatrix} \right\} = 0 \quad \text{for } m \geq 1,$$

$$\bullet \left\{ \begin{smallmatrix} 0 \\ 0 \end{smallmatrix} \right\} = 1$$

Let's look for a recurrence relation:

$$\left\{ \begin{smallmatrix} m \\ k \end{smallmatrix} \right\} = \left\{ \begin{smallmatrix} m-1 \\ k-1 \end{smallmatrix} \right\} + k \left\{ \begin{smallmatrix} m-1 \\ k \end{smallmatrix} \right\} \quad (1)$$

$m$  is in  
a singleton.

for each partition in  $A(m-1, k)$ ,  
we can add  $m$  to any part  
(hence,  $k \cdot |A(m-1, k)|$ ).

Let  $A_k(x) = \sum_{m \geq 0} \left\{ \begin{smallmatrix} m \\ k \end{smallmatrix} \right\} x^m$ . (It's better to cycle over  $m$  since there's  $k \cdot \left\{ \begin{smallmatrix} m-1 \\ k \end{smallmatrix} \right\}$  in (1).)

$$(1) \Rightarrow A_k(x) = x A_{k-1}(x) + k x A_k(x) \Rightarrow$$

$$\Rightarrow A_k(x) = \frac{x^k}{(1-kx) \cdots (1-x)} \underbrace{=}_{\text{partial fractions}} x^k \sum_{r=1}^k (-1)^{k-r} \frac{r^k}{r! (k-r)!} \frac{1}{1-rx}$$

$$\text{Hence, } \left\{ \begin{smallmatrix} m \\ k \end{smallmatrix} \right\} = [x^m] A_k(x) = \frac{1}{k!} \sum_{r=1}^k (-1)^{k-r} \binom{k}{r} r^m$$

$\leadsto k! \left\{ \begin{smallmatrix} m \\ k \end{smallmatrix} \right\} = |\{f: [m] \rightarrow [k] \text{ surjective}\}|$ . Indeed,

each part can be linked bijectively to a number  $j$  in  $[k]$ , hence to get all surjective functions we need to multiply by  $k!$ .

**Exponential generating function (e.g.f.)**

$$\{a_m\}_{m \in \mathbb{N}} \xrightarrow{\text{e.g.f.}} f(x) = \sum_{m \geq 0} \frac{a_m}{m!} x^m$$

$$\{a_{m+h}\}_{m \in \mathbb{N}} \longleftrightarrow D^h f \quad (\text{shifting})$$

**Exercise** Let's use e.g.f.'s to find a formula for  $F_n$ 's

$$F_{m+2} = F_{m+1} + F_m \Rightarrow$$

$$\Rightarrow F'' = F' + F$$

$$\text{Hence } F(x) = \lambda_1 e^{r_+ t} + \lambda_2 e^{r_- t}$$

$$\begin{aligned} x^2 &= x + 1 \Rightarrow \\ \Rightarrow \begin{cases} r_+ &= (1+\sqrt{5})/2 = \varphi \\ r_- &= (1-\sqrt{5})/2 \end{cases} \end{aligned}$$

$$F_0 = 0, F_1 = 1 \Rightarrow$$

$$\Rightarrow \begin{cases} \lambda_1 + \lambda_2 = 0 & (F_0) \\ \lambda_1 r_+ + \lambda_2 r_- = 1 & (F_1) \end{cases} \Rightarrow \begin{cases} \lambda_2 = -\lambda_1 \\ \lambda_1 r_+ - \lambda_1 r_- = 1 \end{cases}$$

$$\leadsto \lambda_1 = \frac{1}{r_+ - r_-} = \frac{1}{\sqrt{5}} \Rightarrow \lambda_2 = -\frac{1}{\sqrt{5}}$$

$$\text{Therefore, } F(x) = \frac{1}{\sqrt{5}} (e^{r_+ t} - e^{r_- t}) \Rightarrow$$

$$\Rightarrow \boxed{F_m = \frac{1}{\sqrt{5}} (r_+^m - r_-^m)} \quad \checkmark$$

- $\{P(m) a_m\} \xleftrightarrow{\text{e.g.f.}} P(xD) f$  (again)

- $f \cdot g \xleftrightarrow{\text{e.g.f.}} \left\{ \sum_{k=0}^m \frac{a_k}{k!} \frac{b_{m-k}}{(m-k)!} m! \right\} = \sum_{k=0}^m \binom{m}{k} a_k b_{m-k}$  (product)

**Example** (Bell numbers)

$$B_0 = 1, B_m \triangleq \# \{ \text{set part of } [m] \} = \sum_{k=0}^m \binom{m}{k}$$

Let  $B(x)$  be  $\{B_m\}$ 's e.g.f. Since  $B_{m+1} = \sum_{k=0}^m \binom{m}{k} B_{m-k}$ ,  
Then:

$$B'(x) = e^x B(x) \Rightarrow$$

$$\Rightarrow B(x) = e^{e^x - 1}$$

cycling over how many el. are in the subset of  $m+1 \in [m+1]$

**Example** (Derangements)

$$D_m \triangleq \# \{ \text{perm} \in S_m \text{ with no fixed points} \}$$

$$D_0 \triangleq 1, D_1 = 0 \text{ Then } |S_m| = m! = \sum_{k=0}^m \underbrace{\binom{m}{k}}_{\text{fixed points}} D_{m-k} \quad (2)$$

$$D(x) \triangleq \sum_{i=0}^{\infty} D_i / i! x^i \text{ (e.g.f.)}$$

From (2) we get  $D(x) \cdot e^x = \frac{1}{1-x} \Rightarrow$

$$\Rightarrow D(x) = \frac{e^{-x}}{1-x} \Rightarrow D_m = m! \left[ \sum_{k=0}^m \frac{(-1)^k}{k!} \right] \left( \Rightarrow D_m = \left\lfloor \frac{m!}{e} \right\rfloor \right)$$

$$D(x) = x D(x) + e^{-x} \Rightarrow D_m = m \cdot D_{m-1} + (-1)^m$$